[minor] Port silent events and new Observation to allocation machine.

pico-ifc-coq/dyn_allocation/AbstractMachine.v
@@ -25,29 +25,29 @@ Definition a_alloc
       (size:Z) (lpc:T) (a:Atom T T) (m:memory T T): option (block T * memory T T) :=
   alloc Local lpc size a m.
 
-Inductive a_step : a_state -> option (Event T) -> a_state -> Prop :=
+Inductive a_step : a_state -> (Event T)+τ -> a_state -> Prop :=
 | step_nop : forall m i s pcv pcl
     (INSTR: index_list_Z pcv i = Some Noop),
-    a_step (AState m i s (pcv,pcl)) None (AState m i s (pcv+1,pcl))
+    a_step (AState m i s (pcv,pcl)) Silent (AState m i s (pcv+1,pcl))
 
 | step_add: forall m i s pcv pcl x1v x1l x2v x2l xv
     (INSTR: index_list_Z pcv i = Some Add)
     (ADD: add x1v x2v = Some xv),
     a_step (AState m i ((AData (x1v,x1l)::(AData (x2v,x2l))::s)) (pcv,pcl))
-               None
+               Silent
                (AState m i ((AData (xv,x1l \_/ x2l))::s) (pcv+1,pcl))
 
 | step_sub: forall m i s pcv pcl x1v x1l x2v x2l xv
     (INSTR: index_list_Z pcv i = Some Sub)
     (SUB: sub x1v x2v = Some xv),
     a_step (AState m i ((AData (x1v,x1l)::(AData (x2v,x2l))::s)) (pcv,pcl))
-               None
+               Silent
                (AState m i ((AData (xv,x1l \_/ x2l))::s) (pcv+1,pcl))
 
 | step_eq: forall m i s pcv pcl x1v x1l x2v x2l
     (INSTR: index_list_Z pcv i = Some Eq),
     a_step (AState m i ((AData (x1v,x1l)::(AData (x2v,x2l))::s)) (pcv,pcl))
-               None
+               Silent
                (AState m i ((AData (val_eq x1v x2v,x1l \_/ x2l))::s) (pcv+1,pcl))
 
 | step_dup : forall m i s1 s2 pcv pcl n x
@@ -55,7 +55,7 @@ Inductive a_step : a_state -> option (Event T) -> a_state -> Prop :=
     (IDX: index_list n s1 = Some x)
     (DATA: forall se, In se s1 -> exists a, se = AData a),
     a_step (AState m i (s1 ++ s2) (pcv, pcl))
-           None
+           Silent
            (AState m i (x :: s1 ++ s2) (pcv+1,pcl))
 
 | step_swap : forall m i s1 s1' s2 pcv pcl n
@@ -63,33 +63,33 @@ Inductive a_step : a_state -> option (Event T) -> a_state -> Prop :=
     (SWAP: swap n s1 = Some s1')
     (DATA: forall se, In se s1 -> exists a, se = AData a),
     a_step (AState m i (s1 ++ s2) (pcv, pcl))
-           None
+           Silent
            (AState m i (s1' ++ s2) (pcv+1,pcl))
 
 | step_push: forall m i s pcv pcl cv
     (INSTR: index_list_Z pcv i = Some (Push cv)),
     a_step (AState m i s (pcv,pcl))
-               None
+               Silent
                (AState m i ((AData (Vint cv,bot))::s) (pcv+1,pcl))
 
 | step_pop: forall m i s pcv pcl a
     (INSTR: index_list_Z pcv i = Some Pop),
     a_step (AState m i (AData a :: s) (pcv,pcl))
-               None
+               Silent
                (AState m i s (pcv+1,pcl))
 
 | step_alloc: forall m i s pcv pcl b size sizel xv xl m'
     (INSTR: index_list_Z pcv i = Some Alloc)
     (ALLOC: a_alloc size (sizel \_/ pcl) (xv,xl) m = Some (b,m')),
     a_step (AState m i ((AData (Vint size,sizel))::(AData (xv,xl))::s) (pcv,pcl))
-               None
+               Silent
                (AState m' i (AData (Vptr b 0,sizel \_/ pcl)::s) (pcv+1,pcl))
 
 | step_load: forall m i s pcv pcl addrl b ofs xv xl
     (INSTR: index_list_Z pcv i = Some Load)
     (LOAD: load b ofs m = Some (xv,xl)),
     a_step (AState m i ((AData (Vptr b ofs,addrl))::s) (pcv,pcl))
-               None
+               Silent
                (AState m i ((AData (xv,addrl \_/ xl)::s)) (pcv+1,pcl))
 
 | step_store: forall m i s pcv pcl b ofs addrl xv xl mv ml m'
@@ -98,26 +98,26 @@ Inductive a_step : a_state -> option (Event T) -> a_state -> Prop :=
     (CHECK: addrl \_/ pcl <: ml = true)
     (STORE: store b ofs (xv, addrl \_/ (xl \_/ pcl)) m = Some m'),
     a_step (AState m i ((AData (Vptr b ofs,addrl))::(AData (xv,xl))::s) (pcv,pcl))
-               None
+               Silent
                (AState m' i s (pcv+1,pcl))
 
 | step_jump: forall m i s pcv pcl pcv' pcl'
     (INSTR: index_list_Z pcv i = Some Jump),
     a_step (AState m i ((AData (Vint pcv',pcl'))::s) (pcv,pcl))
-               None
+               Silent
                (AState m i s (pcv',pcl' \_/ pcl))
 
 | step_branchnz_true: forall m i s pcv pcl offv al
     (INSTR: index_list_Z pcv i = Some (BranchNZ offv)), (* relative target *)
     a_step (AState m i ((AData (Vint 0,al))::s) (pcv,pcl))
-               None
+               Silent
                (AState m i s (pcv+1,al \_/ pcl))
 
 | step_branchnz_false: forall m i s pcv pcl offv av al
     (INSTR: index_list_Z pcv i = Some (BranchNZ offv)) (* relative target *)
     (BRANCH: av <> 0),
     a_step (AState m i ((AData (Vint av,al))::s) (pcv,pcl))
-               None
+               Silent
                (AState m i s (pcv+offv,al \_/ pcl))
 
 | step_call: forall m i s pcv pcl pcv' pcl' args a r
@@ -125,24 +125,24 @@ Inductive a_step : a_state -> option (Event T) -> a_state -> Prop :=
     (LENGTH: length args = a)
     (ARGS: forall a, In a args -> exists d, a = AData d),
     a_step (AState m i ((AData (Vint pcv',pcl'))::args++s) (pcv,pcl))
-               None
+               Silent
                (AState m i (args++(ARet (pcv+1,pcl) r)::s) (pcv',pcl' \_/ pcl))
 
 | step_ret: forall m i s pcv pcl pcv' pcl' s' 
     (INSTR: index_list_Z pcv i = Some Ret)
     (POP: pop_to_return s ((ARet (pcv',pcl') false)::s')),
-    a_step (AState m i s (pcv,pcl)) None (AState m i s' (pcv',pcl'))
+    a_step (AState m i s (pcv,pcl)) Silent (AState m i s' (pcv',pcl'))
 
 | step_vret: forall m i s pcv pcl pcv' pcl' resv resl s' 
     (INSTR: index_list_Z pcv i = Some VRet)
     (POP: pop_to_return s ((ARet (pcv',pcl') true)::s')),
     a_step (AState m i (AData (resv,resl)::s) (pcv,pcl))
-               None (AState m i (AData (resv, resl \_/ pcl)::s') (pcv',pcl'))
+               Silent (AState m i (AData (resv, resl \_/ pcl)::s') (pcv',pcl'))
 
 | step_output: forall m i s pcv pcl xv xl
     (INSTR: index_list_Z pcv i = Some Output),
     a_step (AState m i (AData (Vint xv,xl)::s) (pcv,pcl))
-               (Some (EInt (xv,xl \_/ pcl))) (AState m i s (pcv+1,pcl)).
+               (E (EInt (xv,xl \_/ pcl))) (AState m i s (pcv+1,pcl)).
 
 Lemma a_step_instr : forall m i s pcv pcl s' e,
   a_step (AState m i s (pcv,pcl)) e s' ->
@@ -155,7 +155,7 @@ Qed.
 
 Definition abstract_machine := 
   {| state := a_state ;
-    event := option (Event T) ;
+    event := (Event T) ;
     step := a_step ;
     init_data := abstract_init_data T;
     init_state := fun id =>
