pico-ifc-coq/dyn_allocation/ConcreteMachine.v
@@ -36,13 +36,13 @@ Definition c_alloc (p:privilege) (size:Z) (a:Atom) (m:memory) :=
 (** Concrete machine transition relation.
     Each instructions has 3 semantic rules: (user mode - succ) (user mode - faulting) (kernel mode) *)
 
-Inductive cstep : CS -> option CEvent -> CS -> Prop := 
+Inductive cstep : CS -> CEvent+τ -> CS -> Prop := 
 | cstep_nop : forall m fh i s pcv pcl rl rpcl,
     forall (INST: i @ pcv # Noop)
            (CHIT: cache_hit_mem m (opCodeToZ OpNoop) (__,__,__) pcl)
            (CREAD: cache_hit_read_mem m rl rpcl),
     cstep (CState m fh i s (pcv,pcl) false)
-          None (CState m fh i s (pcv+1,rpcl) false)
+          Silent (CState m fh i s (pcv+1,rpcl) false)
 
 | cstep_nop_f : forall c' m fh i s pcv pcl m',
    forall (INST: i @ pcv # Noop)
@@ -50,11 +50,11 @@ Inductive cstep : CS -> option CEvent -> CS -> Prop :=
           (CUPD: c' = build_cache (opCodeToZ OpNoop) (__,__,__)  pcl)
           (CUPDGET: cupd m c' = Some m'),
     cstep (CState m fh i s (pcv,pcl) false) 
-          None (CState m' fh i ((fh_ret pcv pcl)::s) fh_start true)
+          Silent (CState m' fh i ((fh_ret pcv pcl)::s) fh_start true)
 
 | cstep_nop_p : forall m fh i s pcv pcl,
     fh @ pcv # Noop ->
-    cstep (CState m fh i s (pcv,pcl) true) None (CState m fh i s (pcv+1,handlerTag) true)
+    cstep (CState m fh i s (pcv,pcl) true) Silent (CState m fh i s (pcv+1,handlerTag) true)
 
 | cstep_add: forall fh m i s rpcl pcv pcl rl x1v x1l x2v x2l v,
    forall(INST: i @ pcv # Add)
@@ -62,7 +62,7 @@ Inductive cstep : CS -> option CEvent -> CS -> Prop :=
          (CREAD: cache_hit_read_mem m rl rpcl)
          (ADD: add x1v x2v = Some v),
      cstep (CState m fh i ((x1v,x1l):::(x2v,x2l):::s) (pcv,pcl)    false)  
-           None (CState m fh i          ((v,rl):::s) (pcv+1,rpcl) false)
+           Silent (CState m fh i          ((v,rl):::s) (pcv+1,rpcl) false)
 
 | cstep_add_f: forall c' fh m i s pcv pcl x1v x1l x2v x2l m',
    forall(INST: i @ pcv # Add)
@@ -70,13 +70,13 @@ Inductive cstep : CS -> option CEvent -> CS -> Prop :=
          (CUPD: c' = build_cache (opCodeToZ OpAdd) (x1l,x2l,__)  pcl)
          (CUPDGET: cupd m c' = Some m'),
      cstep (CState m fh i ((x1v,x1l):::(x2v,x2l):::s) (pcv,pcl)    false)  
-           None (CState m' fh i ((fh_ret pcv pcl)::(x1v,x1l):::(x2v,x2l):::s) fh_start true)
+           Silent (CState m' fh i ((fh_ret pcv pcl)::(x1v,x1l):::(x2v,x2l):::s) fh_start true)
 
 | cstep_add_p: forall m fh i s pcv pcl x1v x1l x2v x2l v, 
     fh @ pcv # Add ->
     add x1v x2v = Some v ->
     cstep (CState m fh i ((x1v,x1l):::(x2v,x2l):::s) (pcv,pcl) true)  
-          None (CState m fh i ((v,handlerTag):::s) (pcv+1,handlerTag) true)
+          Silent (CState m fh i ((v,handlerTag):::s) (pcv+1,handlerTag) true)
 
 | cstep_sub: forall fh m i s rpcl pcv  pcl rl x1v x1l x2v x2l v,
    forall(INST: i @ pcv # Sub)
@@ -84,7 +84,7 @@ Inductive cstep : CS -> option CEvent -> CS -> Prop :=
          (CREAD: cache_hit_read_mem m rl rpcl)
          (SUB: sub x1v x2v = Some v),
      cstep (CState m fh i ((x1v,x1l):::(x2v,x2l):::s) (pcv,pcl)    false)  
-           None (CState m fh i          ((v,rl):::s) (pcv+1,rpcl) false)
+           Silent (CState m fh i          ((v,rl):::s) (pcv+1,rpcl) false)
 
 | cstep_sub_f: forall c' fh m i s pcv pcl x1v x1l x2v x2l m',
    forall(INST: i @ pcv # Sub)
@@ -92,20 +92,20 @@ Inductive cstep : CS -> option CEvent -> CS -> Prop :=
          (CUPD: c' = build_cache (opCodeToZ OpSub) (x1l,x2l,__)  pcl)
          (CUPDGET: cupd m c' = Some m'),
      cstep (CState m fh i ((x1v,x1l):::(x2v,x2l):::s) (pcv,pcl)    false)  
-           None (CState m' fh i ((fh_ret pcv pcl)::(x1v,x1l):::(x2v,x2l):::s) fh_start true)
+           Silent (CState m' fh i ((fh_ret pcv pcl)::(x1v,x1l):::(x2v,x2l):::s) fh_start true)
 
 | cstep_sub_p: forall m fh i s pcv pcl x1v x1l x2v x2l v, 
     fh @ pcv # Sub ->
     sub x1v x2v = Some v ->
     cstep (CState m fh i ((x1v,x1l):::(x2v,x2l):::s) (pcv,pcl) true) 
-          None (CState m fh i ((v,handlerTag):::s) (pcv+1,handlerTag) true)
+          Silent (CState m fh i ((v,handlerTag):::s) (pcv+1,handlerTag) true)
 
 | cstep_eq: forall fh m i s rpcl pcv  pcl rl x1v x1l x2v x2l,
    forall(INST: i @ pcv # Eq)
          (CHIT: cache_hit_mem m (opCodeToZ OpEq) (x1l, x2l, __) pcl)
          (CREAD: cache_hit_read_mem m rl rpcl),
      cstep (CState m fh i ((x1v,x1l):::(x2v,x2l):::s) (pcv,pcl)    false)
-           None (CState m fh i          ((val_eq x1v x2v,rl):::s) (pcv+1,rpcl) false)
+           Silent (CState m fh i          ((val_eq x1v x2v,rl):::s) (pcv+1,rpcl) false)
 
 | cstep_eq_f: forall c' fh m i s pcv pcl x1v x1l x2v x2l m',
    forall(INST: i @ pcv # Eq)
@@ -113,32 +113,32 @@ Inductive cstep : CS -> option CEvent -> CS -> Prop :=
          (CUPD: c' = build_cache (opCodeToZ OpEq) (x1l,x2l,__)  pcl)
          (CUPDGET: cupd m c' = Some m'),
      cstep (CState m fh i ((x1v,x1l):::(x2v,x2l):::s) (pcv,pcl)    false)
-           None (CState m' fh i ((fh_ret pcv pcl)::(x1v,x1l):::(x2v,x2l):::s) fh_start true)
+           Silent (CState m' fh i ((fh_ret pcv pcl)::(x1v,x1l):::(x2v,x2l):::s) fh_start true)
 
 | cstep_eq_p: forall m fh i s pcv pcl x1v x1l x2v x2l,
     fh @ pcv # Eq ->
     cstep (CState m fh i ((x1v,x1l):::(x2v,x2l):::s) (pcv,pcl) true)
-          None (CState m fh i ((val_eq x1v x2v,handlerTag):::s) (pcv+1,handlerTag) true)
+          Silent (CState m fh i ((val_eq x1v x2v,handlerTag):::s) (pcv+1,handlerTag) true)
 
 | cstep_dup_p: forall m fh i s pcv pcl n x,
     fh @ pcv # Dup n ->
     index_list n s = Some x ->
     cstep (CState m fh i s (pcv,pcl) true)
-          None (CState m fh i (x::s) (pcv+1,handlerTag) true)
+          Silent (CState m fh i (x::s) (pcv+1,handlerTag) true)
 
 | cstep_swap_p: forall m fh i y s pcv pcl n x s',
     fh @pcv # Swap n -> 
     index_list n (y::s) = Some x ->
     update_list n y (x::s) = Some s' ->
     cstep (CState m fh i (y::s) (pcv,pcl) true)
-          None (CState m fh i s' (pcv+1,handlerTag) true)
+          Silent (CState m fh i s' (pcv+1,handlerTag) true)
 
 | cstep_push: forall fh m i s rpcl pcv pcl rl cv,
    forall(INST: i @ pcv # Push cv)
          (CHIT: cache_hit_mem m (opCodeToZ OpPush) (__ , __, __) pcl)
          (CREAD: cache_hit_read_mem m rl rpcl),
      cstep (CState m fh i s (pcv,pcl)   false)
-           None (CState m fh i ((Vint cv,rl):::s) (pcv+1,rpcl) false)
+           Silent (CState m fh i ((Vint cv,rl):::s) (pcv+1,rpcl) false)
 
 | cstep_push_f: forall c' fh m i s pcv pcl cv m',
    forall(INST : i @ pcv # Push cv)
@@ -146,19 +146,19 @@ Inductive cstep : CS -> option CEvent -> CS -> Prop :=
          (CUPD : c' = build_cache (opCodeToZ OpPush) (__,__,__) pcl)
          (CUPDGET : cupd m c' = Some m'),
      cstep (CState m fh i s (pcv,pcl) false)  
-           None (CState m' fh i ((fh_ret pcv pcl)::s) fh_start true)
+           Silent (CState m' fh i ((fh_ret pcv pcl)::s) fh_start true)
 
 | cstep_push_p: forall m fh i s pcv pcl cv, 
     fh @ pcv # Push cv ->
     cstep (CState m fh i s (pcv,pcl) true) 
-          None (CState m fh i ((Vint cv,handlerTag):::s) (pcv+1,handlerTag) true)
+          Silent (CState m fh i ((Vint cv,handlerTag):::s) (pcv+1,handlerTag) true)
 
 | cstep_pop: forall fh m i s rpcl pcv pcl rl xv xl,
    forall(INST: i @ pcv # Pop)
          (CHIT: cache_hit_mem m (opCodeToZ OpPop) (__ , __, __) pcl)
          (CREAD: cache_hit_read_mem m rl rpcl),
      cstep (CState m fh i ((xv,xl):::s) (pcv,pcl)   false)
-           None (CState m fh i (s) (pcv+1,rpcl) false)
+           Silent (CState m fh i (s) (pcv+1,rpcl) false)
 
 | cstep_pop_f: forall c' fh m i s pcv pcl xv xl m',
    forall(INST : i @ pcv # Pop)
@@ -166,17 +166,17 @@ Inductive cstep : CS -> option CEvent -> CS -> Prop :=
          (CUPD : c' = build_cache (opCodeToZ OpPop) (__,__,__) pcl)
          (CUPDGET : cupd m c' = Some m'),
      cstep (CState m fh i ((xv,xl):::s) (pcv,pcl) false)  
-           None (CState m' fh i ((fh_ret pcv pcl)::(xv,xl):::s) fh_start true)
+           Silent (CState m' fh i ((fh_ret pcv pcl)::(xv,xl):::s) fh_start true)
 
 | cstep_pop_p: forall m fh i s pcv pcl xv xl, 
     fh @ pcv # Pop ->
     cstep (CState m fh i ((xv,xl):::s) (pcv,pcl) true) 
-          None (CState m fh i s (pcv+1,handlerTag) true)
+          Silent (CState m fh i s (pcv+1,handlerTag) true)
 
 | cstep_push_cache_ptr_p: forall m fh i s pcv pcl, 
     fh @ pcv # PushCachePtr ->
     cstep (CState m fh i s (pcv,pcl) true) 
-          None (CState m fh i ((Vptr cblock 0,handlerTag):::s) (pcv+1,handlerTag) true)
+          Silent (CState m fh i ((Vptr cblock 0,handlerTag):::s) (pcv+1,handlerTag) true)
 
 | cstep_alloc: forall fh m i s pcv pcl b size sizel xv xl m' rpcl rl,
                forall (INST: i @ pcv # Alloc)
@@ -184,7 +184,7 @@ Inductive cstep : CS -> option CEvent -> CS -> Prop :=
                       (CREAD: cache_hit_read_mem m rl rpcl)
                       (ALLOC: c_alloc User size (xv,xl) m = Some (b,m')),
                  cstep (CState m fh i (CData (Vint size, sizel)::CData (xv,xl)::s) (pcv,pcl) false)
-                       None
+                       Silent
                        (CState m' fh i (CData (Vptr b 0,rl)::s) (pcv+1,rpcl) false)
 
 | cstep_alloc_f: forall c' fh m m' i s pcv pcl size sizel xv xl,
@@ -193,14 +193,14 @@ Inductive cstep : CS -> option CEvent -> CS -> Prop :=
                         (CUPD: c' = build_cache (opCodeToZ OpAlloc) (sizel, __, __) pcl)
                         (CUPDGET: cupd m c' = Some m'),
                    cstep (CState m fh i (CData (Vint size, sizel)::CData (xv,xl)::s) (pcv,pcl) false)
-                         None
+                         Silent
                          (CState m' fh i (fh_ret pcv pcl::CData (Vint size, sizel)::CData (xv,xl)::s) fh_start true)
 
 | cstep_alloc_p: forall fh m m' i s pcv pcl b size sizel xv xl,
                  forall (INST: fh @ pcv # Alloc)
                         (ALLOC: c_alloc Kernel size (xv,xl) m = Some (b,m')),
                    cstep (CState m fh i (CData (Vint size, sizel)::CData (xv,xl)::s) (pcv,pcl) true)
-                         None
+                         Silent
                          (CState m' fh i (CData (Vptr b 0,handlerTag)::s) (pcv+1,handlerTag) true)
 
 | cstep_load: forall fh m i s rpcl pcv pcl rl b ofs addrl xv xl,
@@ -210,7 +210,7 @@ Inductive cstep : CS -> option CEvent -> CS -> Prop :=
          (MREAD: load b ofs m = Some (xv,xl))
          (PRIV: Mem.stamp b = User),
      cstep (CState m fh i ((Vptr b ofs,addrl):::s) (pcv,pcl)   false)
-           None (CState m fh i ((xv,rl):::s) (pcv+1,rpcl) false)
+           Silent (CState m fh i ((xv,rl):::s) (pcv+1,rpcl) false)
 
 | cstep_load_f: forall c' fh m i s pcv pcl b ofs addrl xv xl m',
    forall(INST: i @ pcv # Load)
@@ -220,14 +220,14 @@ Inductive cstep : CS -> option CEvent -> CS -> Prop :=
          (PRIV: Mem.stamp b = User)
          (CUPDGET : cupd m c' = Some m'),
      cstep (CState m fh i ((Vptr b ofs,addrl):::s) (pcv,pcl)   false)
-           None (CState m' fh i ((fh_ret pcv pcl)::(Vptr b ofs,addrl):::s) fh_start true)
+           Silent (CState m' fh i ((fh_ret pcv pcl)::(Vptr b ofs,addrl):::s) fh_start true)
 
 | cstep_load_p: forall m fh i s pcv pcl b ofs addrl xv xl,
    forall (INST: fh @ pcv # Load)
           (READ: load b ofs m = Some (xv,xl))
           (PRIV: Mem.stamp b = Kernel),
     cstep (CState m fh i ((Vptr b ofs,addrl):::s) (pcv,pcl) true) 
-          None (CState m fh i ((xv,handlerTag):::s) (pcv+1,handlerTag) true)
+          Silent (CState m fh i ((xv,handlerTag):::s) (pcv+1,handlerTag) true)
 
 | cstep_store: forall fh m m' i s rpcl pcv pcl rl b ofs addrl xv xl mv ml,
    forall(INST: i @ pcv # Store)
@@ -237,7 +237,7 @@ Inductive cstep : CS -> option CEvent -> CS -> Prop :=
          (MUPDT: store b ofs (xv,rl) m = Some m')
          (PRIV: Mem.stamp b = User),
      cstep (CState m fh i ((Vptr b ofs,addrl):::(xv,xl):::s) (pcv,pcl)   false)
-           None (CState m' fh i s (pcv+1,rpcl) false)
+           Silent (CState m' fh i s (pcv+1,rpcl) false)
 
 | cstep_store_f: forall c' fh m i s pcv pcl b ofs addrl xv xl mv ml m',
    forall(INST: i @ pcv # Store)
@@ -247,21 +247,21 @@ Inductive cstep : CS -> option CEvent -> CS -> Prop :=
          (PRIV: Mem.stamp b = User)
          (CUPDGET : cupd m c' = Some m'),
      cstep (CState m fh i ((Vptr b ofs,addrl):::(xv,xl):::s) (pcv,pcl)   false)
-           None (CState m' fh i ((fh_ret pcv pcl)::(Vptr b ofs,addrl):::(xv,xl):::s) fh_start true)
+           Silent (CState m' fh i ((fh_ret pcv pcl)::(Vptr b ofs,addrl):::(xv,xl):::s) fh_start true)
 
 | cstep_store_p: forall m fh i s pcv pcl m' b ofs addrl x, 
     forall (INST:fh @ pcv # Store)
            (UPD: store b ofs x m = Some m')
            (PRIV: Mem.stamp b = Kernel),
     cstep (CState m fh i ((Vptr b ofs,addrl)::: x :::s) (pcv,pcl) true)
-          None (CState m' fh i s (pcv+1,handlerTag) true)
+          Silent (CState m' fh i s (pcv+1,handlerTag) true)
 
 | cstep_jump: forall fh m i s rpcl pcv pcl rl cv cl,
    forall(INST: i @ pcv # Jump)
          (CHIT: cache_hit_mem m (opCodeToZ OpJump) (cl, __, __) pcl)
          (CREAD: cache_hit_read_mem m rl rpcl),
      cstep (CState m fh i ((Vint cv,cl):::s) (pcv,pcl)   false)
-           None (CState m fh i s (cv,rpcl) false)
+           Silent (CState m fh i s (cv,rpcl) false)
 
 | cstep_jump_f: forall c' fh m i s pcv pcl cv cl m',
    forall(INST: i @ pcv # Jump)
@@ -269,19 +269,19 @@ Inductive cstep : CS -> option CEvent -> CS -> Prop :=
          (CUPD : c' = build_cache (opCodeToZ OpJump) (cl,__,__) pcl)
          (CUPDGET : cupd m c' = Some m'),
      cstep (CState m fh i ((cv,cl):::s) (pcv,pcl)   false)
-           None (CState m' fh i ((fh_ret pcv pcl)::(cv,cl):::s) fh_start true)
+           Silent (CState m' fh i ((fh_ret pcv pcl)::(cv,cl):::s) fh_start true)
 
 | cstep_jump_p: forall m fh i s pcv pcl pcj pcjl,
     forall (INST: fh @ pcv # Jump),
     cstep (CState m fh i ((Vint pcj,pcjl):::s) (pcv,pcl) true) 
-          None (CState m fh i s (pcj,handlerTag) true)
+          Silent (CState m fh i s (pcj,handlerTag) true)
 
 | cstep_bnz: forall fh m i s rpcl pcv pcl rl cv cl offv,
    forall(INST: i @ pcv # BranchNZ offv)
          (CHIT: cache_hit_mem m (opCodeToZ OpBranchNZ) (cl, __, __) pcl)
          (CREAD: cache_hit_read_mem m rl rpcl),
      cstep (CState m fh i ((Vint cv,cl):::s) (pcv,pcl)   false)
-           None (CState m fh i s (if cv =? 0 then pcv+1 else pcv+offv, rpcl) false)
+           Silent (CState m fh i s (if cv =? 0 then pcv+1 else pcv+offv, rpcl) false)
 
 | cstep_bnz_f: forall c' fh m m' i s pcv pcl cv cl offv,
    forall(INST: i @ pcv # BranchNZ offv)
@@ -289,12 +289,12 @@ Inductive cstep : CS -> option CEvent -> CS -> Prop :=
          (CUPD : c' = build_cache (opCodeToZ OpBranchNZ) (cl,__,__) pcl)
          (CUPDGET: cupd m c' = Some m'),
      cstep (CState m fh i ((Vint cv,cl):::s) (pcv,pcl)   false)
-           None (CState m' fh i ((fh_ret pcv pcl)::(Vint cv,cl):::s) fh_start true)
+           Silent (CState m' fh i ((fh_ret pcv pcl)::(Vint cv,cl):::s) fh_start true)
 
 | cstep_branchnz_p: forall m fh i s pcv pcl offv av al,
     forall (INST: fh @ pcv # BranchNZ offv),
     cstep (CState m fh i ((Vint av,al):::s) (pcv,pcl) true) 
-          None (CState m fh i s (if av =? 0 then pcv+1 else pcv+offv, handlerTag) true)
+          Silent (CState m fh i s (if av =? 0 then pcv+1 else pcv+offv, handlerTag) true)
 
 | cstep_call: forall fh m i s rpcl pcv pcl rl pcc pccl a r args,
    forall(INST: i @ pcv # Call a r)
@@ -303,7 +303,7 @@ Inductive cstep : CS -> option CEvent -> CS -> Prop :=
          (CHIT: cache_hit_mem m (opCodeToZ OpCall) (pccl, __, __) pcl)
          (CREAD: cache_hit_read_mem m rl rpcl),
      cstep (CState m fh i ((Vint pcc,pccl):::args++s) (pcv,pcl)   false)
-           None (CState m fh i (args++(((CRet (pcv+1, rl)) r false)::s)) (pcc,rpcl) false)
+           Silent (CState m fh i (args++(((CRet (pcv+1, rl)) r false)::s)) (pcc,rpcl) false)
 
 | cstep_call_f: forall c' fh m i s pcv pcl pcc pccl a r args m',
    forall(INST: i @ pcv # Call a r)
@@ -313,14 +313,14 @@ Inductive cstep : CS -> option CEvent -> CS -> Prop :=
          (CUPD : c' = build_cache (opCodeToZ OpCall) (pccl,__,__) pcl)
          (CUPDGET : cupd m c' = Some m'),
      cstep (CState m fh i ((pcc,pccl):::args++s) (pcv,pcl)   false)
-           None (CState m' fh i ((fh_ret pcv pcl)::(pcc,pccl):::args++s) fh_start true)
+           Silent (CState m' fh i ((fh_ret pcv pcl)::(pcc,pccl):::args++s) fh_start true)
 
 | cstep_call_p: forall m fh i s pcv pcl a r args pcc pccl,
     forall (INST: fh @ pcv # Call a r)
            (ARGSA: length args = a)
            (ARGS: forall a, In a args -> exists d, a = CData d),
     cstep (CState m fh i ((Vint pcc,pccl):::args++s) (pcv,pcl) true) 
-          None (CState m fh i (args++(CRet (pcv+1, pcl) r true)::s) (pcc, handlerTag) true)
+          Silent (CState m fh i (args++(CRet (pcv+1, pcl) r true)::s) (pcc, handlerTag) true)
 
 | cstep_ret: forall fh m i s s' pcv pcl rl rpcl pcret pcretl,
    forall(INST: i @ pcv # Ret)
@@ -329,7 +329,7 @@ Inductive cstep : CS -> option CEvent -> CS -> Prop :=
                 (*DD: should only return to user mode *)
          (CREAD: cache_hit_read_mem m rl rpcl),
      cstep (CState m fh i s  (pcv,pcl) false)
-           None (CState m fh i s' (pcret, rpcl) false)
+           Silent (CState m fh i s' (pcret, rpcl) false)
 
 | cstep_ret_f: forall c' fh m i s' s pcv pcl pret pcret pcretl m',
    forall(INST: i @ pcv # Ret)
@@ -340,13 +340,13 @@ Inductive cstep : CS -> option CEvent -> CS -> Prop :=
          (CUPD : c' = build_cache (opCodeToZ OpRet) (pcretl,__,__) pcl)
          (CUPDGET : cupd m c' = Some m'),
      cstep (CState m fh i s  (pcv,pcl) false)
-           None (CState m' fh i ((fh_ret pcv pcl)::s) fh_start true)
+           Silent (CState m' fh i ((fh_ret pcv pcl)::s) fh_start true)
 
 | cstep_ret_p: forall m fh i s pcv pcl  pcret pcretl s' pret, 
     forall (INST: fh @ pcv # Ret) (* can either return to user/priv mode *)
            (POP: c_pop_to_return s ((CRet (pcret,pcretl) false pret)::s')),
     cstep (CState m fh i s  (pcv,pcl) true) 
-          None (CState m fh i s' (pcret,pcretl) pret)
+          Silent (CState m fh i s' (pcret,pcretl) pret)
 
 | cstep_vret: forall fh m i s s' pcv pcl rl rpcl resv resl pcret pcretl,
    forall(INST: i @ pcv # VRet)
@@ -355,7 +355,7 @@ Inductive cstep : CS -> option CEvent -> CS -> Prop :=
                 (*DD: should only return to user mode *)
          (CREAD: cache_hit_read_mem m rl rpcl),
      cstep (CState m fh i ((resv,resl):::s)  (pcv,pcl) false)
-           None (CState m fh i ((resv,rl):::s') (pcret,rpcl) false)
+           Silent (CState m fh i ((resv,rl):::s') (pcret,rpcl) false)
 
 | cstep_vret_f: forall c' fh m i s' s pcv pcl resv resl pcret pcretl m',
    forall(INST: i @ pcv # VRet)
@@ -364,20 +364,20 @@ Inductive cstep : CS -> option CEvent -> CS -> Prop :=
          (CUPD : c' = build_cache (opCodeToZ OpVRet) (resl,pcretl,__) pcl)
          (CUPDGET : cupd m c' = Some m'),
      cstep (CState m fh i ((resv,resl):::s)  (pcv,pcl) false)
-           None (CState m' fh i ((fh_ret pcv pcl)::(resv,resl):::s) fh_start true)
+           Silent (CState m' fh i ((fh_ret pcv pcl)::(resv,resl):::s) fh_start true)
 
 | cstep_vret_p: forall m fh i s pcv pcl s' pcret pcretl resv resl, 
     forall (INST: fh @ pcv # VRet) (* cannot vreturn to user mode *)
            (POP: c_pop_to_return s ((CRet (pcret,pcretl) true true)::s')),
     cstep (CState m fh i ((resv,resl):::s) (pcv,pcl) true) 
-          None (CState m fh i ((resv,resl):::s') (pcret, pcretl) true)
+          Silent (CState m fh i ((resv,resl):::s') (pcret, pcretl) true)
 
 | cstep_out: forall fh m i s rpcl pcv pcl rl cv cl,
    forall(INST: i @ pcv # Output)
          (CHIT: cache_hit_mem m (opCodeToZ OpOutput) (cl, __, __) pcl)
          (CREAD: cache_hit_read_mem m rl rpcl),
      cstep (CState m fh i ((Vint cv,cl):::s) (pcv,pcl)   false)
-           (Some (CEInt (cv,rl))) (CState m fh i s (pcv+1,rpcl) false)
+           (E (CEInt (cv,rl))) (CState m fh i s (pcv+1,rpcl) false)
 
 | cstep_out_f: forall c' fh m i s pcv pcl cv cl m',
    forall(INST: i @ pcv # Output)
@@ -385,7 +385,7 @@ Inductive cstep : CS -> option CEvent -> CS -> Prop :=
          (CUPD : c' = build_cache (opCodeToZ OpOutput) (cl,__,__) pcl)
          (CUPDGET : cupd m c' = Some m'),
      cstep (CState m fh i ((Vint cv,cl):::s) (pcv,pcl)   false)
-           None (CState m' fh i ((fh_ret pcv pcl)::(Vint cv,cl):::s) fh_start true).
+           Silent (CState m' fh i ((fh_ret pcv pcl)::(Vint cv,cl):::s) fh_start true).
 
 Definition initial_memory : memory :=
   (* Once again, it is OK to start with an empty cache. This will
@@ -395,7 +395,7 @@ Definition initial_memory : memory :=
 
 Definition concrete_machine (faultHandler: list Instr) : semantics := 
   {| state := CS ;
-    event := option CEvent ;
+    event := CEvent ;
     step := cstep ;
     init_data := list Instr * list PcAtom * Z;
     init_state := fun id => 
@@ -411,7 +411,7 @@ Definition concrete_machine (faultHandler: list Instr) : semantics :=
 Lemma priv_no_event_l : forall s e s'
                                (STEP : cstep s e s')
                                (PRIV : priv s = true),
-                          e = None.
+                          e = Silent.
 Proof.
   intros.
   inv STEP; simpl in *; try congruence; auto.
@@ -420,7 +420,7 @@ Qed.
 Lemma priv_no_event_r : forall s e s'
                                (STEP : cstep s e s')
                                (PRIV : priv s' = true),
-                          e = None.
+                          e = Silent.
 Proof.
   intros.
   inv STEP; simpl in *; try congruence; auto.
