pico-ifc-coq/dyn_allocation/Semantics.v
@@ -1,9 +1,11 @@
+Require Import Utils.
+
 Set Implicit Arguments.
 
 Record semantics :=
 {   state : Type 
   ; event : Type 
-  ; step : state -> event -> state -> Prop
+  ; step : state -> event+τ -> state -> Prop
   ; init_data : Type
   ; init_state : init_data -> state
 }.
